retrieve done

theories/lang/lang.v
@@ -459,8 +459,8 @@ Definition write_retrieve_msg (st:state) (dst: Addr) (wh:handle) (trn: transacti
   | (vs, f, _ ,vr, ls, t) =>
     match finz.of_z (Z.of_nat (length ls)) with
     | Some l =>
-      let des := ([of_imm (encode_vmid vs); f; wh; encode_transaction_type t ;l;
-                                       of_imm (encode_vmid vr)] ++ map of_pid ls) in
+      let des := ([of_imm (encode_vmid vs); f; wh; encode_transaction_type t ;l]
+                    ++ map of_pid ls) in
       match finz.of_z (Z.of_nat (length des)) with
       | Some l' => fill_rx (write_mem_segment_unsafe st dst des) l' vr vr
       | None => throw InvParam
@@ -713,21 +713,27 @@ Definition retrieve (s : state) : exec_mode * state :=
       match m with
       | (vs, Some handle, _, _, _) =>
         trn <- lift_option_with_err (get_transaction s handle) InvParam ;;;
-        (let (r, ps) := get_memory_descriptor trn in
-         let ty := get_transaction_type trn in
-         s' <- (write_retrieve_msg s (get_rx_pid_global s (get_current_vm s)) handle trn) ;;;
-         (* for all pages of the trancation ... (change the page table of the caller according to the type)*)
-         match ty with
-         | Sharing =>
-           s'' <- toggle_transaction_retrieve s' handle trn ;;;
-           unit (update_access_batch (update_reg s'' R0 (encode_hvc_ret_code Succ)) ps SharedAccess)
-         | Lending =>
-           s'' <- toggle_transaction_retrieve s' handle trn ;;;
-           (* it is fine because we only allow at most one receiver *)
-           unit (update_access_batch (update_reg s'' R0 (encode_hvc_ret_code Succ)) ps ExclusiveAccess)
-         | Donation =>
-           unit (update_access_batch (update_ownership_batch (update_reg (remove_transaction s' handle) R0 (encode_hvc_ret_code Succ)) ps Owned) ps ExclusiveAccess)
-         end)
+        match get_transaction s handle with
+         | Some (vs, w1, b,r, ps, ty) =>
+           match ((get_current_vm s) =? r) , b  with
+           | true, false =>
+             s' <- (write_retrieve_msg s (get_rx_pid_global s (get_current_vm s)) handle trn) ;;;
+             match ty with
+             | Sharing =>
+               unit (update_access_batch (update_reg (update_transaction s' handle (vs, w1, true ,r, ps, ty))
+                                                     R0 (encode_hvc_ret_code Succ)) ps SharedAccess)
+             | Lending =>
+               (* it is fine because we only allow at most one receiver *)
+               unit (update_access_batch (update_reg (update_transaction s' handle (vs, w1, true ,r, ps, ty))
+                                                     R0 (encode_hvc_ret_code Succ)) ps ExclusiveAccess)
+             | Donation =>
+               unit (update_access_batch (update_ownership_batch (update_reg (remove_transaction s' handle)
+                                                R0 (encode_hvc_ret_code Succ)) ps Owned) ps ExclusiveAccess)
+             end
+           | _ , _ => throw Denied
+           end
+         | None => throw InvParam
+         end
       | _ => throw InvParam
       end
   in
