theories/rules/retrieve.v
@@ -25,7 +25,7 @@ Lemma hvc_retrieve_donate_nz {wi sown sacc pi sexcl i j destx wf' desrx ptx prx 
   spsd ## sexcl ->
   (finz.to_z l) = Z.of_nat (length psd) ->
   destx = ([of_imm (encode_vmid j); wf'; wh ;of_imm (encode_vmid i)] ) ->
-  desrx = ([of_imm (encode_vmid j); wf; wh; l;encode_transaction_type Donation ; of_imm (encode_vmid i)] ++ map of_pid psd) ->
+  desrx = ([of_imm (encode_vmid j); wf; wh; encode_transaction_type Donation;l] ++ map of_pid psd) ->
   (finz.to_z r1) = (Z.of_nat (length destx)) ->
   seq_in_page (of_pid ptx) (length destx) ptx ->
   seq_in_page (of_pid prx) (length desrx) prx ->
@@ -38,7 +38,7 @@ Lemma hvc_retrieve_donate_nz {wi sown sacc pi sexcl i j destx wf' desrx ptx prx 
    ExecI @ i {{{ RET ExecI ; PC @@ i ->r (ai ^+ 1)%f ∗ ai ->a wi
   ∗ O@i:={1}[(sown ∪ spsd)] ∗ E@i:={1}[(sexcl ∪ spsd)] ∗ A@i:={1}[(sacc ∪ spsd)]
   ∗ R0 @@ i ->r (encode_hvc_ret_code Succ) ∗ R1 @@ i ->r r1
-  ∗ TX@ i := ptx ∗ RX@ i :=( prx ! r1, i)
+  ∗ TX@ i := ptx ∗ RX@ i :=( prx ! (l ^+ 5)%f, i)
   ∗ mem_region destx ptx ∗ mem_region desrx prx
   ∗ hp{ 1 }[ sh ∪ {[wh]} ] }}}.
 Proof.
@@ -89,33 +89,45 @@ Proof.
       done.
       contradiction.
     }
+    assert (Hlendesclt' :((Z.of_nat (length desrx)) <= (page_size-1))%Z).
+    {
+      destruct Hseqrx as [? [HisSome Hltpagesize]].
+      apply (finz_plus_Z_le (of_pid prx)); eauto.
+      apply last_addr_in_bound.
+      apply Z.leb_le.
+      destruct (((prx ^+ length desrx)%f <=? (prx ^+ (page_size - 1))%f)%Z).
+      done.
+      contradiction.
+    }
     destruct (page_size <? r1)%Z eqn:Hr1ps; [lia|].
     rewrite /get_tx_pid_global Hcureq Htx in Heqc2.
     rewrite (@transaction_retrieve_descriptor_valid j wh wf' σ1 destx ptx) /= in Heqc2; eauto.
     2: { rewrite Hcureq; auto. }
     rewrite Htrans /= in Heqc2.
     rewrite -Hlenl finz_of_z_to_z in Heqc2.
-    assert (finz.of_z (Z.of_nat (S (S (S (S (S (S (length (map of_pid psd))))))))) = Some (l ^+ 6%Z)%f).
+    assert (finz.of_z (Z.of_nat (S (S (S (S (S (length (map of_pid psd)))))))) = Some (l ^+ 5%Z)%f).
     {  rewrite Hdesrx in Hseqrx. destruct Hseqrx as [_ [HisSome Hltpagesize]]. cbn in HisSome, Hltpagesize.
-       assert (Heq: Z.of_nat(S (S (S (S (S (S (length (map of_pid psd))))))))
-               = ((Z.of_nat (length (map of_pid psd))) + 6%Z)%Z).
+       assert (Heq: Z.of_nat(S (S (S (S (S (length (map of_pid psd)))))))
+                    = ((Z.of_nat (length (map of_pid psd))) + 5%Z)%Z).
        lia.
        rewrite Heq map_length.
        rewrite -Hlenl.
        rewrite Heq map_length -Hlenl in Hltpagesize.
        rewrite Heq map_length -Hlenl in HisSome.
        pose proof (last_addr_in_bound prx).
-       assert (Hle:( (finz.to_z l + 6)%Z <= (page_size-1)%Z)%Z).
+       assert (Hle:( (finz.to_z l + 5)%Z <= (page_size-1)%Z)%Z).
        apply (finz_plus_Z_le (of_pid prx));auto.
-       apply Z.leb_le. destruct ((((of_pid prx) ^+ (finz.to_z l + 6)%Z)%f <=?((of_pid prx) ^+ (page_size-1)%Z)%f)%Z) eqn:Heqn;[done|contradiction].
+       apply Z.leb_le.
+       destruct ((((of_pid prx) ^+ (finz.to_z l + 5)%Z)%f <=?((of_pid prx) ^+ (page_size-1)%Z)%f)%Z)
+                eqn:Heqn;[done|contradiction].
        unfold finz.of_z.
-       destruct (decide (finz.to_z l + 6 < word_size)%Z) eqn:Hdecide.
+       destruct (decide (finz.to_z l + 5 < word_size)%Z) eqn:Hdecide.
        unfold decide  in Hdecide.
        unfold decide_rel in Hdecide.
        rewrite Hdecide.
        2: {  lia. }
        clear Hdecide.
-       destruct (decide (0<= finz.to_z l + 6 )%Z) eqn:Hdecide.
+       destruct (decide (0<= finz.to_z l + 5 )%Z) eqn:Hdecide.
        unfold decide  in Hdecide.
        unfold decide_rel in Hdecide.
        rewrite Hdecide /=.
@@ -124,7 +136,7 @@ Proof.
        apply finz_to_z_eq.
        cbn.
        solve_finz.
-   }
+    }
     rewrite H in Heqc2. clear H.
     rewrite /fill_rx in Heqc2.
     assert (Htemp : ∀ σ dst ws i, get_vm_mail_box (write_mem_segment_unsafe σ dst ws) i =
@@ -133,21 +145,22 @@ Proof.
     rewrite Htemp in Heqc2; clear Htemp.
     assert (Hmb :  get_vm_mail_box σ1 i = (ptx, (prx,None))).
     { destruct (get_vm_mail_box σ1 i).
-    destruct r.
-    cbn in Htx ,Hrx2, Hrx1.
-    subst t0 o p.
-    reflexivity.
+      destruct r.
+      cbn in Htx ,Hrx2, Hrx1.
+      subst t0 o p.
+      reflexivity.
     }
     rewrite /get_tx_pid_global /get_rx_pid_global Hmb /=  in Heqc2.
-    (* assert (Hcheck : (i =? i)%nat = true). *)
-    (* { by apply <- Nat.eqb_eq. } *)
-    (* rewrite Hcheck in Heqc2. *)
-    (* pose proof Hretri1 as Hretri1''. *)
-    (* pose proof Hretri2 as Hretri2''. *)
-    (* rewrite Htrans in Hretri1. *)
-    (* inversion Hretri1 as [Hretri1']. *)
-    (* rewrite -Hretri1' //= in Hretri2. *)
-    (* rewrite Hretri2 //= /transaction_write_rx /transaction_to_list_words /transaction_to_transaction_descriptor in Heqc2. *)
+    assert (Hcheck: (i =? i)%nat = true).
+    { apply <- Nat.eqb_eq. reflexivity. }
+    rewrite Hcheck in Heqc2.
+    pose proof Hretri1 as Hretri1'.
+    pose proof Hretri2 as Hretri2'.
+    rewrite Htrans in Hretri1.
+    inversion Hretri1 as [Hretri1''].
+    rewrite -Hretri1'' //= in Hretri2.
+    subst b t.
+    clear Hretri2' Hretri1.
     destruct c2 as [c21 c22].
     destruct HstepP; subst m2 σ2; rewrite Heqc2.
     simpl;clear Heqc2.
@@ -168,36 +181,36 @@ Proof.
     rewrite update_offset_PC_preserve_rx1 update_access_batch_preserve_rx1 update_ownership_batch_preserve_rx1
             update_reg_global_preserve_rx1 remove_transaction_preserve_rx1 fill_rx_unsafe_preserve_rx1.
     rewrite  write_mem_segment_unsafe_preserve_rx1.
-     2 : {
-       rewrite /get_rx_pid_global /get_vm_mail_box /get_mail_boxes //=.
-     }
-     iFrame "Hσrx1".
+    2 : {
+      rewrite /get_rx_pid_global /get_vm_mail_box /get_mail_boxes //=.
+    }
+    iFrame "Hσrx1".
     (* update regs *)
     rewrite (update_offset_PC_update_PC1 _ i ai 1).
     rewrite update_access_batch_preserve_regs update_ownership_batch_preserve_regs
             update_reg_global_update_reg remove_transaction_preserve_regs
-             fill_rx_unsafe_preserve_regs write_mem_segment_unsafe_preserve_regs; try solve_reg_lookup.
+            fill_rx_unsafe_preserve_regs write_mem_segment_unsafe_preserve_regs; try solve_reg_lookup.
     2:{
       rewrite update_access_batch_preserve_current_vm update_ownership_batch_preserve_current_vm
               update_reg_global_preserve_current_vm remove_transaction_preserve_current_vm
-       fill_rx_unsafe_preserve_current_vm write_mem_segment_unsafe_preserve_current_vm //.
+              fill_rx_unsafe_preserve_current_vm write_mem_segment_unsafe_preserve_current_vm //.
     }
     2: {
       rewrite update_access_batch_preserve_regs update_ownership_batch_preserve_regs
               update_reg_global_update_reg remove_transaction_preserve_regs
-             fill_rx_unsafe_preserve_regs write_mem_segment_unsafe_preserve_regs; try solve_reg_lookup.
+              fill_rx_unsafe_preserve_regs write_mem_segment_unsafe_preserve_regs; try solve_reg_lookup.
       rewrite lookup_insert_ne; [solve_reg_lookup|done].
     }
-     iDestruct ((gen_reg_update2_global PC i _ (ai ^+ 1)%f R0 i _ (encode_hvc_ret_code Succ)) with "Hσreg PC Hr0")
+    iDestruct ((gen_reg_update2_global PC i _ (ai ^+ 1)%f R0 i _ (encode_hvc_ret_code Succ)) with "Hσreg PC Hr0")
       as ">[Hσreg [PC Hr0]]";try f_equal.
     { left;done. }
-     iFrame "Hσreg".
+    iFrame "Hσreg".
     (* update page table *)
     rewrite update_offset_PC_preserve_owned update_access_batch_preserve_ownerships.
     rewrite (@update_ownership_batch_update_pagetable_union _ i sown spsd psd Hpsd); f_equal;eauto.
     iDestruct ((gen_own_update_union spsd) with "HO Hσowned") as ">[Hσowned HO]";f_equal.
     exact Hpsd.
-     rewrite update_reg_global_preserve_owned remove_transaction_preserve_owned
+    rewrite update_reg_global_preserve_owned remove_transaction_preserve_owned
             fill_rx_unsafe_preserve_owned write_mem_segment_unsafe_preserve_owned.
     iFrame "Hσowned".
     rewrite update_offset_PC_preserve_access.
@@ -207,7 +220,7 @@ Proof.
     rewrite update_ownership_batch_preserve_access update_reg_global_preserve_access remove_transaction_preserve_access
     fill_rx_unsafe_preserve_access write_mem_segment_unsafe_preserve_access.
     2: { rewrite update_ownership_batch_preserve_access update_reg_global_preserve_access remove_transaction_preserve_access
-    fill_rx_unsafe_preserve_access write_mem_segment_unsafe_preserve_access. done. }
+                 fill_rx_unsafe_preserve_access write_mem_segment_unsafe_preserve_access. done. }
     iFrame "Hσaccess".
     rewrite update_offset_PC_preserve_excl.
     rewrite (@update_exclusive_batch_update_pagetable_union _ i sexcl spsd psd Hpsd);f_equal; eauto.
@@ -216,100 +229,265 @@ Proof.
     rewrite update_ownership_batch_preserve_excl update_reg_global_preserve_excl remove_transaction_preserve_excl
     fill_rx_unsafe_preserve_excl write_mem_segment_unsafe_preserve_excl.
     2: { rewrite update_ownership_batch_preserve_excl update_reg_global_preserve_excl remove_transaction_preserve_excl
-    fill_rx_unsafe_preserve_excl write_mem_segment_unsafe_preserve_excl. done. }
+                 fill_rx_unsafe_preserve_excl write_mem_segment_unsafe_preserve_excl. done. }
     iFrame "Hσexcl".
     (* update rx *)
-    iCombine "HRX1 HRX2" as "HRX".
     rewrite update_offset_PC_preserve_rx2 update_access_batch_preserve_rx2 update_ownership_batch_preserve_rx2
             update_reg_global_preserve_rx2 remove_transaction_preserve_rx2.
-    iDestruct ((gen_rx_gmap_update_global_None i r1 i prx) with "Hσrx2 HRX") as ">[Hσrx' [HRX1 HRX2]]".
+    iDestruct ((gen_rx_gmap_update_global_None i (l ^+ 5)%f i prx) with "Hσrx2 [HRX1 HRX2]") as ">[Hσrx' [HRX1 HRX2]]".
+    { iFrame. }
     rewrite fill_rx_unsafe_update_mailbox write_mem_segment_unsafe_preserve_rx2.
     iFrame "Hσrx'".
-
-    (* TODO  *)
-
-
-    (* rewrite update_offset_PC_preserve_hpool update_access_batch_preserve_hpool *)
-    (*         update_reg_global_preserve_hpool update_transaction_preserve_hpool fill_rx_unsafe_preserve_hpool *)
-    (*         write_segment_unsafe_preserve_hpool. *)
-    (* iFrame "Hσhp". *)
-
-
     (* update transactions *)
     rewrite -get_trans_gmap_preserve_dom.
     rewrite update_offset_PC_preserve_trans update_access_batch_preserve_trans
-            update_ownership_batch_preserve_trans update_reg_global_preserve_trans.
-    rewrite (@toggle_transaction_unsafe_preserve_trans _ _ b).
-    2 : {
-      cbn.
-      assumption.
-    }
-    rewrite fill_rx_unsafe_preserve_trans copy_page_segment_unsafe_preserve_trans.
+            update_ownership_batch_preserve_trans update_reg_global_preserve_trans
+            remove_transaction_update_trans fill_rx_unsafe_preserve_trans
+            write_mem_segment_unsafe_preserve_trans.
+    iDestruct (gen_trans_update_delete with "Hwh Htrans") as ">Htrans".
     iFrame "Htrans".
-      (* update retri *)
-    rewrite update_offset_PC_preserve_mem update_access_batch_preserve_mem
-            update_reg_global_preserve_mem update_transaction_preserve_mem fill_rx_unsafe_preserve_mem.
-    iDestruct ((@gen_retri_update _ _ _ false true wh) with "Hwhf Hrcv") as ">[Hrcv' Hwhf']".
-    { subst b t.
-      eapply get_retri_gmap_lookup.
-      exact Hretri1''.
-    }
-    rewrite update_offset_PC_preserve_retri update_access_batch_preserve_retri
-    update_reg_global_preserve_retri /update_transaction /insert_transaction.
-    rewrite -get_retri_gmap_to_get_transaction fill_rx_unsafe_preserve_receivers
-    copy_page_segment_unsafe_preserve_receivers.
-    iFrame "Hrcv'".
-    rewrite update_offset_PC_preserve_trans' update_access_batch_preserve_trans'
-            update_reg_global_preserve_trans' /get_transactions /=.
-    (* update mem *)
-    rewrite /copy_page_segment_unsafe /copy_from_addr_to_addr_unsafe.
-    rewrite /mem_region.
-    assert (Hlength: ((read_mem_segment_unsafe σ1 ptx r1)) = des).
+    (* update hpool *)
+    rewrite update_offset_PC_preserve_hpool update_access_batch_preserve_hpool
+            update_ownership_batch_preserve_hpool update_reg_global_preserve_hpool
+            remove_transaction_update_hpool fill_rx_unsafe_preserve_hpool
+            write_mem_segment_unsafe_preserve_hpool.
+    iDestruct ((gen_hpool_update_union wh) with "Hpool Hσhp") as ">[Hσhp Hpool]".
     {
-      rewrite /read_mem_segment_unsafe.
-      rewrite /get_mem in Hadesc.
-      apply (f_equal Z.to_nat) in Hdesl.
-      rewrite Hdesl.
-      rewrite Nat2Z.id.
-      clear Hdes Hdesl Hseq Hlendesclt Hmb.
-      generalize dependent (of_pid ptx).
-      induction des; first done.
-      simpl in IHdes.
-      simpl.
-      intros.
-      rewrite /get_memory_unsafe.
-      rewrite (Hadesc 0 f a).
-      simpl.
-      f_equal.
-      rewrite /get_memory_unsafe in IHdes.
-      rewrite (IHdes (f ^+ 1)%f).
-      reflexivity.
-      intros k y1 y2 H1 H2.
-      apply Hadesc with (S k); auto.
-      reflexivity.
-      reflexivity.
+      rewrite /get_hpool_gset.
+      unfold get_fresh_handles in Hpool.
+      assert (Hwhin : wh ∈ dom (gset handle) (get_transactions σ1).1).
+      {
+        apply elem_of_dom.
+        eexists.
+        done.
+      }
+      set_solver.
     }
+    iFrame "Hσhp".
+    (* update retri *)
+    rewrite update_offset_PC_preserve_mem update_access_batch_preserve_mem
+            update_ownership_batch_preserve_mem update_reg_global_preserve_mem
+            remove_transaction_preserve_mem fill_rx_unsafe_preserve_mem.
+    iDestruct ((gen_retri_update_delete wh) with "Hwhf Hrcv") as ">Hrcv";auto.
+    rewrite update_offset_PC_preserve_trans' update_access_batch_preserve_trans'
+            update_ownership_batch_preserve_trans'
+            update_reg_global_preserve_trans' /get_transactions /=.
+    rewrite update_offset_PC_preserve_retri update_access_batch_preserve_retri
+            update_ownership_batch_preserve_retri update_reg_global_preserve_retri
+            remove_transaction_update_retri fill_rx_unsafe_preserve_receivers
+            write_mem_segment_unsafe_preserve_receivers.
+    iFrame "Hrcv".
+    (* update mem *)
+    rewrite /write_mem_segment_unsafe /mem_region.
     iDestruct "HRXCont" as "[%l0 [HRXCont' %Hlen']]".
-    rewrite Hlength.
-    rewrite /write_mem_segment_unsafe //.
     cbn.
-    iDestruct ((gen_mem_update_SepL2 (finz.seq rxp (length l0)) l0 des) with "Hσmem HRXCont'")
+    iDestruct ((gen_mem_update_SepL2 (finz.seq prx (length l0)) l0 desrx) with "Hσmem HRXCont'")
       as ">[Hσmem Hmem]".
     { rewrite Hlen'.
       apply finz_seq_NoDup'.
-      pose proof last_addr_in_bound as Hbound.
-      specialize (Hbound rxp).
+      pose proof (last_addr_in_bound prx).
       solve_finz.
     }
     assumption.
-    assert ((zip (finz.seq rxp (length l0)) des) = (zip (finz.seq rxp (Z.to_nat 1000)) des)) as ->.
+    assert ((zip (finz.seq prx (length l0)) desrx) = (zip (finz.seq prx (Z.to_nat 1000)) desrx)) as ->.
     {
       rewrite -finz_seq_zip_page;auto.
       rewrite Hlen' //.
       lia.
     }
+    cbn in Hdesrx.
+    rewrite -Hdesrx.
     iFrame "Hσmem".
     iSplitR.
+    iPureIntro.
+    split;[rewrite dom_delete get_trans_gmap_preserve_dom;set_solver |].
+    apply map_Forall_delete; auto.
+    iApply "HΦ".
+    rewrite Hlen'.
+    by iFrame.
+Qed.
+
+
+Lemma retrieve_lend_share {sacc sexcl j desrx ptx prx l ai r0 wh wf} σ1 i tt sexcl' acc (spsd: gset PID)
+       (psd: list PID):
+  tt = Lending ∧ sexcl' = sexcl ∪ spsd ∧ acc = ExclusiveAccess ∨ tt = Sharing ∧ sexcl' = sexcl ∧ acc = SharedAccess ->
+  spsd = list_to_set psd ->
+  finz.to_z l = Z.of_nat (length psd) ->
+  desrx = [of_imm (encode_vmid j); wf; wh; encode_transaction_type tt; l] ++ map of_pid psd ->
+  seq_in_page (of_pid prx) (length desrx) prx ->
+  (get_vm_mail_box σ1 i).1 = ptx ->
+  (get_vm_mail_box σ1 i).2.1 = prx ->
+  (get_current_vm σ1) = i ->
+  get_reg σ1 PC = Some ai ->
+  get_reg σ1 R0 = Some r0 ->
+  spsd ## sacc ->
+  spsd ## sexcl ->
+  (get_transactions σ1).1 !! wh = Some (j, wf, false, i, psd, tt) ->
+  PC @@ i ->r ai -∗
+  A@i:={1}[sacc] -∗
+  E@i:={1}[sexcl] -∗
+  R0 @@ i ->r r0 -∗
+  wh->t{1}(j,wf,i,psd,tt) -∗
+  wh->refalse -∗
+  RX@i:=prx -∗
+  rx_option_mapsto i None -∗
+  (∃ l0 : list handle, mem_region l0 prx ∗ ⌜length l0 = length desrx⌝) -∗
+  gen_vm_interp σ1 ={⊤}=∗
+  gen_vm_interp (update_incr_PC
+            (update_access_batch
+               (update_reg
+                  (update_transaction
+                     (fill_rx_unsafe
+                        (write_mem_segment_unsafe σ1 (of_pid prx)
+                           ( of_imm (encode_vmid j) :: wf :: wh :: encode_transaction_type tt :: l :: map of_pid psd))
+                        (l ^+ 5)%f i i ptx prx) wh (j, wf, true, i, psd, tt)) R0
+                  (encode_hvc_ret_code Succ)) psd acc))
+  ∗ wh->t{1}(j,wf,i,psd,tt)
+  ∗ PC @@ i ->r (ai ^+ 1)%f
+  ∗ R0 @@ i ->r encode_hvc_ret_code Succ
+  ∗ RX@i:=prx
+  ∗ rx_option_mapsto i (Some ((l ^+ 5)%f, i))
+  ∗ wh->retrue
+  ∗ ([∗ list] a;w' ∈ finz.seq prx (length desrx);(of_imm (encode_vmid j) :: wf :: wh :: encode_transaction_type tt
+                                                              :: l :: map of_pid psd), a ->a w')
+  ∗ A@i:={1}[sacc ∪ spsd]
+  ∗ E@i:={1}[sexcl'].
+Proof.
+  iIntros (Htt Hpsd Hlenl Hdesrx Hseqrx Htx Hrx1 Hcureq HPC HR1 Hsacc Hsexcl Htrans) "PC Hacc Hexcl R0 Htrans Hretri Hrx1 Hrx2 Hmemdesrx Hσ".
+  iDestruct "Hσ" as "(Hcur & Hσmem & Hσreg & Hσtx & Hσrx1 & Hσrx2 & Hσowned & Hσaccess & Hσexcl
+          & Hσtrans & Hσhp & %Hdisj & %Hlen & Hσretri)".
+  iDestruct ((gen_access_valid_pure sacc) with "Hσaccess Hacc") as %Hacc; eauto.
+  iDestruct ((gen_excl_valid_pure sexcl) with "Hσexcl Hexcl") as %Hexcl; eauto.
+  rewrite /gen_vm_interp /update_incr_PC /update_reg.
+  rewrite update_offset_PC_preserve_hpool update_access_batch_preserve_hpool
+          update_reg_global_preserve_hpool update_transaction_preserve_hpool fill_rx_unsafe_preserve_hpool
+          write_mem_segment_unsafe_preserve_hpool.
+  iFrame "Hσhp".
+  rewrite update_offset_PC_preserve_tx update_access_batch_preserve_tx
+          update_reg_global_preserve_tx update_transaction_preserve_tx fill_rx_unsafe_preserve_tx.
+  2 : {
+    rewrite /get_tx_pid_global /get_vm_mail_box //= /get_mail_boxes.
+  }
+  rewrite write_mem_segment_unsafe_preserve_tx.
+  rewrite /get_tx_agree.
+  iFrame "Hσtx".
+  rewrite update_offset_PC_preserve_current_vm update_access_batch_preserve_current_vm
+          update_reg_global_preserve_current_vm update_transaction_preserve_current_vm
+          fill_rx_unsafe_preserve_current_vm write_mem_segment_unsafe_preserve_current_vm.
+  rewrite Hcureq.
+  iFrame "Hcur".
+  rewrite update_offset_PC_preserve_rx1 update_access_batch_preserve_rx1
+          update_reg_global_preserve_rx1 update_transaction_preserve_rx1.
+  rewrite fill_rx_unsafe_preserve_rx1.
+  2 : {
+    rewrite /get_rx_pid_global /get_vm_mail_box /get_mail_boxes //=.
+  }
+  rewrite write_mem_segment_unsafe_preserve_rx1.
+  iFrame "Hσrx1".
+  (* update regs *)
+  rewrite (update_offset_PC_update_PC1 _ i ai 1).
+  rewrite update_access_batch_preserve_regs update_reg_global_update_reg update_transaction_preserve_regs
+          fill_rx_unsafe_preserve_regs write_mem_segment_unsafe_preserve_regs; try solve_reg_lookup.
+  2:{
+    rewrite update_access_batch_preserve_current_vm update_reg_global_preserve_current_vm
+            update_transaction_preserve_current_vm fill_rx_unsafe_preserve_current_vm
+            write_mem_segment_unsafe_preserve_current_vm //.
+  }
+  2: {
+    rewrite update_access_batch_preserve_regs update_reg_global_update_reg.
+    rewrite update_transaction_preserve_regs
+            fill_rx_unsafe_preserve_regs write_mem_segment_unsafe_preserve_regs; try solve_reg_lookup.
+    rewrite lookup_insert_ne; [solve_reg_lookup|done].
+    exists r0.
+    rewrite update_transaction_preserve_regs
+            fill_rx_unsafe_preserve_regs write_mem_segment_unsafe_preserve_regs; try solve_reg_lookup.
+  }
+  iDestruct ((gen_reg_update2_global PC i _ (ai ^+ 1)%f R0 i _ (encode_hvc_ret_code Succ)) with "Hσreg PC R0")
+    as ">[Hσreg [PC R0]]";try f_equal.
+  { left;done. }
+  iFrame "Hσreg".
+  (* update transactions *)
+  rewrite -get_trans_gmap_preserve_dom.
+  rewrite update_offset_PC_preserve_trans update_access_batch_preserve_trans
+          update_reg_global_preserve_trans (update_transaction_preserve_trans _ _ false).
+  2 : { cbn. assumption. }
+  rewrite fill_rx_unsafe_preserve_trans write_mem_segment_unsafe_preserve_trans.
+  iFrame "Hσtrans".
+  (* update rx *)
+  iCombine "Hrx1 Hrx2" as "Hrx".
+  rewrite update_offset_PC_preserve_rx2 update_access_batch_preserve_rx2
+          update_reg_global_preserve_rx2 update_transaction_preserve_rx2.
+  iDestruct ((gen_rx_gmap_update_global_None i (l ^+ 5)%f i prx) with "Hσrx2 Hrx") as ">[Hσrx [Hrx1 Hrx2]]".
+  rewrite fill_rx_unsafe_update_mailbox.
+  iFrame "Hσrx".
+  (* update retri *)
+  rewrite update_offset_PC_preserve_mem update_access_batch_preserve_mem
+          update_reg_global_preserve_mem update_transaction_preserve_mem fill_rx_unsafe_preserve_mem.
+  iDestruct ((@gen_retri_update _ _ _ false true wh) with "Hretri Hσretri") as ">[Hσretri Hretri]".
+  {
+    eapply get_retri_gmap_lookup.
+    exact Htrans.
+  }
+  rewrite update_offset_PC_preserve_retri update_access_batch_preserve_retri
+  update_reg_global_preserve_retri update_transaction_update_retri
+  fill_rx_unsafe_preserve_receivers write_mem_segment_unsafe_preserve_receivers.
+  iFrame "Hσretri".
+  rewrite update_offset_PC_preserve_trans' update_access_batch_preserve_trans'
+          update_reg_global_preserve_trans' /get_transactions /=.
+  (* update mem *)
+  rewrite /write_mem_segment_unsafe /mem_region.
+  iDestruct "Hmemdesrx" as "[%l0 [Hmemdesrx %Hlen']]".
+  cbn.
+   assert (Hlendesrxle: ((Z.of_nat (length desrx)) <= (page_size-1))%Z).
+    {
+      destruct Hseqrx as [? [HisSome Hltpagesize]].
+      apply (finz_plus_Z_le (of_pid prx)); eauto.
+      apply last_addr_in_bound.
+      apply Z.leb_le.
+      destruct (((prx ^+ length desrx)%f <=? (prx ^+ (page_size - 1))%f)%Z).
+      done.
+      contradiction.
+    }
+  iDestruct ((gen_mem_update_SepL2 (finz.seq prx (length l0)) l0 desrx) with "Hσmem Hmemdesrx")
+    as ">[Hσmem Hmem]".
+  { rewrite Hlen'.
+    apply finz_seq_NoDup'.
+    pose proof (last_addr_in_bound prx).
+        solve_finz.
+  }
+  assumption.
+  assert ((zip (finz.seq prx (length l0)) desrx) = (zip (finz.seq prx (Z.to_nat 1000)) desrx)) as ->.
+  {
+    rewrite -finz_seq_zip_page;auto.
+    rewrite Hlen' //.
+    lia.
+  }
+  cbn in Hdesrx.
+  rewrite Hdesrx.
+  iFrame "Hσmem".
+  (* update page table *)
+  rewrite update_offset_PC_preserve_owned update_access_batch_preserve_ownerships
+          update_reg_global_preserve_owned update_transaction_preserve_owned
+          fill_rx_unsafe_preserve_owned write_mem_segment_unsafe_preserve_owned.
+  iFrame "Hσowned".
+  rewrite update_offset_PC_preserve_access.
+  destruct Htt as [(-> & ->& ->)|(-> & ->& ->)].
+  {
+    rewrite (@update_access_batch_update_pagetable_union _ i sacc ExclusiveAccess spsd psd Hpsd); f_equal;eauto.
+    iDestruct ((gen_access_update_union spsd) with "Hacc Hσaccess") as ">[Hσaccess Hacc]";f_equal.
+    {exact Hpsd. }
+    rewrite update_reg_global_preserve_access update_transaction_preserve_access
+    fill_rx_unsafe_preserve_access write_mem_segment_unsafe_preserve_access.
+    iFrame "Hσaccess".
+    rewrite update_offset_PC_preserve_excl.
+    rewrite (@update_exclusive_batch_update_pagetable_union _ i sexcl spsd psd Hpsd);f_equal; eauto.
+    iDestruct ((gen_excl_update_union spsd) with "Hexcl Hσexcl") as ">[Hσexcl Hexcl]"; f_equal.
+    { exact Hpsd. }
+    rewrite update_reg_global_preserve_excl update_transaction_preserve_excl
+    fill_rx_unsafe_preserve_excl write_mem_segment_unsafe_preserve_excl.
+    iFrame "Hσexcl".
+    rewrite Hlen' -Hdesrx.
+    iFrame "Htrans PC R0 Hrx1 Hrx2 Hretri Hmem Hacc Hexcl".
     iPureIntro.
     split;[rewrite get_trans_gmap_preserve_dom // |].
     apply map_Forall_insert_2; auto.
@@ -318,273 +496,46 @@ Proof.
     destruct (finz_spec word_size l) as [H _].
     rewrite ->(reflect_iff _ _ (Z.ltb_spec0 l word_size)) in H.
     assumption.
-    iApply "HΦ".
-    rewrite Hlen'.
-    by iFrame.
-Qed.
-
-
-
-
-
-
-
-
-
-
-
-
-    rewrite (@transaction_retrieve_descriptor_valid j wh wf l psd σ1 destx ptx) /= in Heqc2; eauto.
-    2: { rewrite Hcureq; auto. }
-    rewrite Htrans /= in Heqc2.
-    rewrite /transfer_msg /transfer_msg_unsafe Hr1ps //= /get_current_vm //= /get_vm_mail_box /get_mail_boxes //in Heqc2.
-    rewrite /get_vm_mail_box /get_mail_boxes in Htx Hrx2.
-    pose proof (surjective_pairing (σ1.1.1.1.1.2 !!! i)) as Hpair.
-    rewrite (surjective_pairing (σ1.1.1.1.1.2 !!! i).2) in Hpair.
-    rewrite Htx Hrx1 Hrx2 in Hpair.
-    rewrite //= /fill_rx /get_vm_mail_box /get_mail_boxes // /get_mail_boxes // in Heqc2.
-    rewrite Hpair //= in Heqc2.
-    destruct HstepP; subst m2 σ2; subst c2; simpl.
-    rewrite /gen_vm_interp /update_incr_PC /update_reg.
-    rewrite update_offset_PC_preserve_current_vm
-            update_access_batch_preserve_current_vm
-            update_ownership_batch_preserve_current_vm
-            update_reg_global_preserve_current_vm
-            remove_transaction_preserve_current_vm
-            fill_rx_unsafe_preserve_current_vm
-            copy_page_segment_unsafe_preserve_current_vm.
-    cbn.
-    iFrame "Hcur".
-    rewrite update_offset_PC_preserve_tx
-            update_access_batch_preserve_tx
-            update_ownership_batch_preserve_tx
-            update_reg_global_preserve_tx
-            remove_transaction_preserve_tx
-            fill_rx_unsafe_preserve_tx.
-    2 : {
-      rewrite /get_tx_pid_global /get_vm_mail_box //= /get_mail_boxes.
-    }
-    rewrite copy_page_segment_unsafe_preserve_tx.
-    rewrite /get_tx_agree.
-    iFrame "Hσtx".
-    rewrite update_offset_PC_preserve_rx1
-            update_access_batch_preserve_rx1
-            update_ownership_batch_preserve_rx1
-            update_reg_global_preserve_rx1
-            remove_transaction_preserve_rx1
-            fill_rx_unsafe_preserve_rx1.
-    rewrite copy_page_segment_unsafe_preserve_rx1.
-    iFrame "Hσrx1".
-    (* update regs *)
-    rewrite (update_offset_PC_update_PC1 _ i ai 1).
-    rewrite update_access_batch_preserve_regs update_ownership_batch_preserve_regs update_reg_global_update_reg.
-    rewrite remove_transaction_preserve_regs fill_rx_unsafe_preserve_regs copy_page_segment_unsafe_preserve_regs;
-      try solve_reg_lookup.
-    2 : {
-      exists r0.
-      rewrite get_reg_gmap_get_reg_Some.
-      rewrite /get_reg /get_reg_global /get_vm_reg_file /get_reg_files //= Hcureq /get_current_vm //= in HR0 *.
-      f_equal.
-    }
-    2 : {
-      rewrite update_access_batch_preserve_current_vm
-              update_ownership_batch_preserve_current_vm
-              update_reg_global_preserve_current_vm
-              remove_transaction_preserve_current_vm
-              fill_rx_unsafe_preserve_current_vm
-              copy_page_segment_unsafe_preserve_current_vm.
-      rewrite Hcureq.
-      reflexivity.
-    }
-    2: {
-      rewrite update_access_batch_preserve_regs update_ownership_batch_preserve_regs update_reg_global_update_reg.
-      (* try solve_reg_lookup. *)
-      rewrite !lookup_insert_ne; [|done].
-      rewrite get_reg_gmap_get_reg_Some.
-      rewrite /get_reg /get_reg_global /get_vm_reg_file /get_reg_files //= ?Hcureq /get_current_vm //= in HPC *.
-      rewrite <-Hcureq.
-      f_equal.
-      exists r0.
-      rewrite get_reg_gmap_get_reg_Some; auto.
-    }
-    2 : {
-      rewrite /copy_page_segment_unsafe /get_rx_pid_global /copy_from_addr_to_addr_unsafe /write_mem_segment_unsafe
-              /update_memory_global_batch /get_vm_mail_box /get_mail_boxes.
-      cbn.
-      rewrite Hpair.
-      reflexivity.
-    }
-     iDestruct ((gen_reg_update2_global PC i _ (ai ^+ 1)%f R0 i _ (encode_hvc_ret_code Succ)) with "Hσreg PC Hr0")
-      as ">[Hσreg [PC Hr0]]";try f_equal.
-    { left; done. }
-    rewrite Hcureq.
-     iFrame "Hσreg".
-    (* update page table *)
-    rewrite update_offset_PC_preserve_owned
-            update_access_batch_preserve_ownerships.
-    rewrite update_offset_PC_preserve_access.
-    rewrite (@update_ownership_batch_update_pagetable_union _ i sown spsd psd Hpsd); f_equal;eauto.
-    iDestruct ((gen_own_update_union spsd) with "HO Hσowned") as ">[Hσown' HO']"; f_equal.
-    { exact Hpsd. }
-    iFrame "Hσown'".
-    rewrite (@update_access_batch_update_pagetable_union _ i sacc ExclusiveAccess spsd psd Hpsd); f_equal;eauto.
-    iDestruct ((gen_access_update_union spsd) with "HA Hσaccess") as ">[Hσaccess' HA']";f_equal.
-    { exact Hpsd. }
-    rewrite update_ownership_batch_preserve_access update_reg_global_preserve_access remove_transaction_preserve_access
-            fill_rx_unsafe_preserve_access copy_page_segment_unsafe_preserve_access.
-    iFrame "Hσaccess'".
-    2 : {
-        by rewrite update_ownership_batch_preserve_access
-                   update_reg_global_preserve_access remove_transaction_preserve_access
-                   fill_rx_unsafe_preserve_access copy_page_segment_unsafe_preserve_access.
-    }
-    rewrite update_offset_PC_preserve_excl.
-    rewrite (@update_exclusive_batch_update_pagetable_union _ i sexcl spsd psd Hpsd); f_equal; eauto.
-    iDestruct ((gen_excl_update_union spsd) with "HE Hσexcl") as ">[Hσexcl' HE']"; f_equal.
-    { exact Hpsd. }
-    rewrite update_ownership_batch_preserve_excl update_reg_global_preserve_excl remove_transaction_preserve_excl
-            fill_rx_unsafe_preserve_excl copy_page_segment_unsafe_preserve_excl.
-    iFrame "Hσexcl'".
-    2 : {
-        by rewrite update_ownership_batch_preserve_excl update_reg_global_preserve_excl remove_transaction_preserve_excl
-                   fill_rx_unsafe_preserve_excl copy_page_segment_unsafe_preserve_excl.
+  }
+  {
+    rewrite (@update_access_batch_update_pagetable_union _ i sacc SharedAccess spsd psd Hpsd); f_equal;eauto.
+    iDestruct ((gen_access_update_union spsd) with "Hacc Hσaccess") as ">[Hσaccess Hacc]";f_equal.
+    {exact Hpsd. }
+    rewrite update_reg_global_preserve_access update_transaction_preserve_access
+    fill_rx_unsafe_preserve_access write_mem_segment_unsafe_preserve_access.
+    iFrame "Hσaccess".
+    rewrite update_offset_PC_preserve_excl (@update_access_batch_preserve_excl spsd sexcl);auto.
+    2: { rewrite update_reg_global_preserve_excl update_transaction_preserve_excl
+    fill_rx_unsafe_preserve_excl write_mem_segment_unsafe_preserve_excl.
+     rewrite update_reg_global_preserve_current_vm update_transaction_preserve_current_vm
+    fill_rx_unsafe_preserve_current_vm write_mem_segment_unsafe_preserve_current_vm Hcureq //.
      }
-    (* update transactions *)
-    rewrite update_offset_PC_preserve_trans
-            update_access_batch_preserve_trans update_ownership_batch_preserve_trans
-            update_reg_global_preserve_trans.
-    rewrite remove_transaction_update_trans.
-    rewrite fill_rx_unsafe_preserve_trans copy_page_segment_unsafe_preserve_trans.
-    iDestruct (gen_trans_update_delete with "Hwh Htrans") as ">Htrans".
-    iFrame "Htrans".
-     (* update rx *)
-    iCombine "HRX1 HRX2" as "HRX".
-    iEval (rewrite -Hcureq) in "HRX".
-    iDestruct ((gen_rx_gmap_update_global_None (get_current_vm σ1) r1 (get_current_vm σ1) rxp) with "Hσrx2 HRX") as ">[Hσrx' [HRX1 HRX2]]".
-    rewrite update_offset_PC_preserve_rx2
-            update_access_batch_preserve_rx2
-            update_ownership_batch_preserve_rx2
-            update_reg_global_preserve_rx2
-            remove_transaction_preserve_rx2.
-    rewrite fill_rx_unsafe_update_mailbox.
-    rewrite copy_page_segment_unsafe_preserve_rx2.
-    iEval (rewrite -Hcureq /get_current_vm) in "Hσrx'".
-    rewrite -Hcureq.
-    iFrame "Hσrx'".
-    (* update mem *)
-    rewrite update_offset_PC_preserve_mem update_access_batch_preserve_mem
-            update_ownership_batch_preserve_mem update_reg_global_preserve_mem
-            remove_transaction_preserve_mem fill_rx_unsafe_preserve_mem.
-    rewrite /copy_page_segment_unsafe /copy_from_addr_to_addr_unsafe.
-    rewrite /get_tx_pid_global /get_vm_mail_box /get_mail_boxes //=.
-    rewrite -Hcureq /get_current_vm in Htx.
-    rewrite Htx.
-    rewrite /mem_region.
-    assert (Hlength: ((read_mem_segment_unsafe σ1 ptx r1)) = des).
-    {
-      rewrite /read_mem_segment_unsafe.
-      rewrite /get_mem in Hadesc.
-      apply (f_equal Z.to_nat) in Hdesl.
-      rewrite Hdesl.
-      rewrite Nat2Z.id.
-      clear Hdes Hdesl Hseq Hlendesclt Htx Hpair.
-      generalize dependent (of_pid ptx).
-      induction des; first done.
-      simpl in IHdes.
-      simpl.
-      intros.
-      rewrite /get_memory_unsafe.
-      rewrite (Hadesc 0 f a).
-      simpl.
-      f_equal.
-      rewrite /get_memory_unsafe in IHdes.
-      rewrite (IHdes (f ^+ 1)%f).
-      reflexivity.
-      intros k y1 y2 H1 H2.
-      apply Hadesc with (S k); auto.
-      reflexivity.
-      reflexivity.
-    }
-    iDestruct "HRXCont" as "[%l0 [HRXCont' %Hlen']]".
-    rewrite Hlength.
-    rewrite /write_mem_segment_unsafe //.
-    rewrite /get_rx_pid_global /get_vm_mail_box /get_mail_boxes.
-    rewrite -Hcureq in Hpair.
-    rewrite Hpair.
-    cbn.
-    iDestruct ((gen_mem_update_SepL2 (finz.seq rxp (length l0)) l0 des) with "Hσmem HRXCont'") as ">[Hmemupd1 Hmemupd2]".
-    rewrite Hlen'.
-    apply finz_seq_NoDup'.
-    pose proof last_addr_in_bound as Hbound.
-    specialize (Hbound rxp).
-    solve_finz.
-    assumption.
-    assert ((zip (finz.seq rxp (length l0)) des) = (zip (finz.seq rxp (Z.to_nat 1000)) des)) as  -> .
-    {
-      rewrite -finz_seq_zip_page;auto.
-      rewrite Hlen' //.
-      lia.
-    }
-    iFrame "Hmemupd1".
-    rewrite update_offset_PC_preserve_retri update_access_batch_preserve_retri
-            update_ownership_batch_preserve_retri update_reg_global_preserve_retri.
-    iDestruct ((gen_retri_update_delete wh) with "Hwhf Hrcv") as ">Hrcv".
-    rewrite remove_transaction_update_retri.
-    rewrite fill_rx_unsafe_preserve_receivers.
-    assert (∀ σ l, get_retri_gmap (update_memory_global_batch σ l) = get_retri_gmap σ) as ->. f_equal.
-    iFrame "Hrcv".
-    iCombine "Hpool Hσhp" as "Hhp".
-    iDestruct ((@gen_hpool_update_union _ _ σ1 sh 1 wh) with "Hhp") as ">[Hσhp' Hpool']".
-    {
-      rewrite /get_hpool_gset.
-      rewrite /get_fresh_handles in Hpool.
-      intros contra.
-      assert (contra' : wh ∉ dom (gset handle) (get_transactions σ1).1).
-      {
-        symmetry in Hdisj.
-        rewrite ->elem_of_disjoint in Hdisj.
-        specialize (Hdisj wh contra).
-        auto.
-      }
-      apply contra'.
-      apply elem_of_dom.
-      exists t.
-      auto.
-    }
-    rewrite update_offset_PC_preserve_hpool update_access_batch_preserve_hpool
-            update_ownership_batch_preserve_hpool update_reg_global_preserve_hpool.
-    rewrite remove_transaction_update_hpool.
-    rewrite fill_rx_unsafe_preserve_hpool.
-    assert (∀ σ l, get_hpool_gset (update_memory_global_batch σ l) = get_hpool_gset σ) as ->. f_equal.
-    iFrame "Hσhp'".
-    iSplitR.
+    rewrite update_reg_global_preserve_excl update_transaction_preserve_excl
+    fill_rx_unsafe_preserve_excl write_mem_segment_unsafe_preserve_excl.
+    iFrame "Hσexcl".
+    rewrite Hlen' -Hdesrx.
+    iFrame "Htrans PC R0 Hrx1 Hrx2 Hretri Hmem Hacc Hexcl".
     iPureIntro.
-    rewrite update_offset_PC_preserve_trans'
-            update_access_batch_preserve_trans'
-            update_ownership_batch_preserve_trans'
-            update_reg_global_preserve_trans'.
-    rewrite /get_transactions.
-    cbn.
-    split.
-    rewrite dom_delete.
-    rewrite disjoint_union_r.
-    split.
-    apply disjoint_difference_l2; auto.
-    apply disjoint_difference_l1; auto.
-    apply map_Forall_delete; auto.
-    iApply "HΦ".
-    rewrite Hlen'.
-    by iFrame.
+    split;[rewrite get_trans_gmap_preserve_dom // |].
+    apply map_Forall_insert_2; auto.
+    simpl.
+    rewrite <-Hlenl.
+    destruct (finz_spec word_size l) as [H _].
+    rewrite ->(reflect_iff _ _ (Z.ltb_spec0 l word_size)) in H.
+    assumption.
+  }
 Qed.
 
-Lemma hvc_retrieve_lend_nz {wi sown sacc pi sexcl i j des ptx rxp l} {spsd: gset PID}
+
+Lemma hvc_retrieve_lend_share {tt sexcl' wi sown sacc pi sexcl i j destx wf' desrx ptx prx l} {spsd: gset PID}
       ai r0 r1 wh wf (psd: list PID) :
   (* the current instruction is hvc *)
   (* the decoding of wi is correct *)
   decode_instruction wi = Some(Hvc) ->
+  tt = Lending ∧ sexcl' = (sexcl ∪ spsd) ∨ tt = Sharing ∧ sexcl' = sexcl->
   (* the instruction is in page pi *)
   addr_in_page ai pi ->
-  (* the decoding of R0 is FFA_LEND *)
+  (* the decoding of R0 is FFA_RETRIEVE *)
   decode_hvc_func r0 = Some(Retrieve) ->
   (* pi page in spsd is accessible for VM i *)
   pi ∈ sacc ->
@@ -594,22 +545,24 @@ Lemma hvc_retrieve_lend_nz {wi sown sacc pi sexcl i j des ptx rxp l} {spsd: gset
   spsd ## sown ->
   spsd ## sexcl ->
   (finz.to_z l) = (Z.of_nat (length psd)) ->
-  des = ([of_imm (encode_vmid j); wf; wh; l; of_imm (encode_vmid i)] ++ map of_pid psd) ->
-  (finz.to_z r1) = (Z.of_nat (length des)) ->
-  seq_in_page (of_pid ptx) (length des) ptx ->
+  destx = ([of_imm (encode_vmid j); wf'; wh ;of_imm (encode_vmid i)] ) ->
+  desrx = ([of_imm (encode_vmid j); wf; wh; encode_transaction_type tt;l] ++ map of_pid psd) ->
+  (finz.to_z r1) = (Z.of_nat (length destx)) ->
+  seq_in_page (of_pid ptx) (length destx) ptx ->
+  seq_in_page (of_pid prx) (length desrx) prx ->
   {SS{{ ▷(PC @@ i ->r ai) ∗ ▷ ai ->a wi ∗ ▷ A@i:={1}[sacc]
   ∗ ▷ (R0 @@ i ->r r0) ∗ ▷ wh ->re false
-  ∗ ▷ (R1 @@ i ->r r1) ∗ ▷ wh ->t{1}(j, wf, i, psd, Lending)
+  ∗ ▷ (R1 @@ i ->r r1) ∗ ▷ wh ->t{1}(j, wf, i, psd, tt)
   ∗ ▷ O@i:={1}[sown] ∗ ▷ E@i:={1}[sexcl] ∗ ▷ TX@ i := ptx
-  ∗ ▷ mem_region des ptx ∗ ▷ RX@ i :=( rxp !) ∗ ▷ (∃l, mem_region l rxp ∗ ⌜ length l = length des ⌝)}}}
+  ∗ ▷ mem_region destx ptx ∗ ▷ RX@ i :=( prx !) ∗ ▷ (∃l, mem_region l prx ∗ ⌜ length l = length desrx ⌝)}}}
    ExecI @ i {{{ RET ExecI ; PC @@ i ->r (ai ^+ 1)%f ∗ ai ->a wi
-  ∗ O@i:={1}[(sown)] ∗ E@i:={1}[(sexcl ∪ spsd)] ∗ A@i:={1}[(sacc ∪ spsd)]
-  ∗ R0 @@ i ->r (encode_hvc_ret_code Succ) ∗ R1 @@ i ->r r1 ∗ wh ->t{1}(j, wf, i, psd, Lending)
-  ∗ wh ->re true ∗ TX@ i := ptx ∗ RX@ i :=( rxp ! r1, i)
-  ∗ mem_region des ptx ∗ mem_region des rxp }}}.
+  ∗ O@i:={1}[(sown)] ∗ E@i:={1}[sexcl'] ∗ A@i:={1}[(sacc ∪ spsd)]
+  ∗ R0 @@ i ->r (encode_hvc_ret_code Succ) ∗ R1 @@ i ->r r1 ∗ wh ->t{1}(j, wf, i, psd, tt)
+  ∗ wh ->re true ∗ TX@ i := ptx ∗ RX@ i :=( prx ! (l ^+ 5)%f, i)
+  ∗ mem_region destx ptx ∗ mem_region desrx prx }}}.
 Proof.
-  iIntros (Hdecodei Hinpi Hdecodef Hpiacc Hpsd Hsown Hsacc Hsexcl Hlenl Hdes Hdesl Hseq Φ).
-  iIntros "(>PC & >Hai & >HA & >Hr0 & >Hwhf & >Hr1 & >Hwh & >HO & >HE & >HTX & >Hmemr & >HRX & >HRXCont) HΦ".
+  iIntros (Hdecodei Htt Hinpi Hdecodef Hpiacc Hpsd Hsown Hsacc Hsexcl Hlenl Hdestx Hdesrx Hdestxl Hseqtx Hseqrx).
+  iIntros (Φ) "(>PC & >Hai & >HA & >Hr0 & >Hwhf & >Hr1 & >Hwh & >HO & >HE & >HTX & >Hmemr & >HRX & >HRXCont) HΦ".
   iApply (sswp_lift_atomic_step ExecI); [done|].
   iIntros (σ1) "%Hsche Hσ".
   inversion Hsche as [Hcureq]; clear Hsche.
@@ -626,8 +579,8 @@ Proof.
   destruct Htrans as [b Htrans].
   iDestruct (gen_retri_valid with "Hwhf Hrcv") as %Hretri.
   destruct Hretri as [t [Hretri1 Hretri2]].
-  iDestruct (gen_mem_valid_SepL_pure _ des with "Hσmem Hmemr") as %Hadesc.
-  { apply finz_seq_NoDup. destruct Hseq as [? [HisSome ?]]. done. }
+  iDestruct (gen_mem_valid_SepL_pure _ destx with "Hσmem Hmemr") as %Hadesc.
+  { apply finz_seq_NoDup. destruct Hseqtx as [? [HisSome ?]]. done. }
   iDestruct (gen_tx_valid with "HTX Hσtx") as %Htx.
   iDestruct (gen_rx_valid_none with "HRX Hσrx2") as %Hrx2.
   iDestruct "HRX" as "(HRX1 & HRX2)".
@@ -644,213 +597,208 @@ Proof.
     apply (step_ExecI_normal i Hvc ai wi) in HstepP; eauto.
     remember (exec Hvc σ1) as c2 eqn:Heqc2.
     rewrite /exec /hvc HR0 Hdecodef /retrieve /get_transaction HR1 //= in Heqc2.
-    assert (Hlendesclt :((Z.of_nat (length des)) <= (page_size-1))%Z).
+    assert (Hlendesclt :((Z.of_nat (length destx)) <= (page_size-1))%Z).
     {
-      destruct Hseq as [? [HisSome Hltpagesize]].
+      destruct Hseqtx as [? [HisSome Hltpagesize]].
       apply (finz_plus_Z_le (of_pid ptx)); eauto.
       apply last_addr_in_bound.
       apply Z.leb_le.
-      destruct (((ptx ^+ length des)%f <=? (ptx ^+ (page_size - 1))%f)%Z).
+      destruct (((ptx ^+ length destx)%f <=? (ptx ^+ (page_size - 1))%f)%Z).
+      done.
+      contradiction.
+    }
+    assert (Hlendesclt' :((Z.of_nat (length desrx)) <= (page_size-1))%Z).
+    {
+      destruct Hseqrx as [? [HisSome Hltpagesize]].
+      apply (finz_plus_Z_le (of_pid prx)); eauto.
+      apply last_addr_in_bound.
+      apply Z.leb_le.
+      destruct (((prx ^+ length desrx)%f <=? (prx ^+ (page_size - 1))%f)%Z).
       done.
       contradiction.
     }
     destruct (page_size <? r1)%Z eqn:Hr1ps; [lia|].
     rewrite /get_tx_pid_global Hcureq Htx in Heqc2.
-    rewrite (@transaction_retrieve_descriptor_valid j wh wf l psd σ1 des ptx) /= in Heqc2; eauto.    
+    rewrite (@transaction_retrieve_descriptor_valid j wh wf' σ1 destx ptx) /= in Heqc2; eauto.
     2: { rewrite Hcureq; auto. }
     rewrite Htrans /= in Heqc2.
-    rewrite /transfer_msg Hcureq in Heqc2.
-    rewrite /transfer_msg_unsafe Hr1ps in Heqc2.
+    rewrite -Hlenl finz_of_z_to_z in Heqc2.
+    assert (finz.of_z (Z.of_nat (S (S (S (S (S (length (map of_pid psd)))))))) = Some (l ^+ 5%Z)%f).
+    {  rewrite Hdesrx in Hseqrx. destruct Hseqrx as [_ [HisSome Hltpagesize]]. cbn in HisSome, Hltpagesize.
+       assert (Heq: Z.of_nat(S (S (S (S (S (length (map of_pid psd)))))))
+                    = ((Z.of_nat (length (map of_pid psd))) + 5%Z)%Z).
+       lia.
+       rewrite Heq map_length.
+       rewrite -Hlenl.
+       rewrite Heq map_length -Hlenl in Hltpagesize.
+       rewrite Heq map_length -Hlenl in HisSome.
+       pose proof (last_addr_in_bound prx).
+       assert (Hle:( (finz.to_z l + 5)%Z <= (page_size-1)%Z)%Z).
+       apply (finz_plus_Z_le (of_pid prx));auto.
+       apply Z.leb_le.
+       destruct ((((of_pid prx) ^+ (finz.to_z l + 5)%Z)%f <=?((of_pid prx) ^+ (page_size-1)%Z)%f)%Z)
+                eqn:Heqn;[done|contradiction].
+       unfold finz.of_z.
+       destruct (decide (finz.to_z l + 5 < word_size)%Z) eqn:Hdecide.
+       unfold decide  in Hdecide.
+       unfold decide_rel in Hdecide.
+       rewrite Hdecide.
+       2: {  lia. }
+       clear Hdecide.
+       destruct (decide (0<= finz.to_z l + 5 )%Z) eqn:Hdecide.
+       unfold decide  in Hdecide.
+       unfold decide_rel in Hdecide.
+       rewrite Hdecide /=.
+       2: {  lia. }
+       f_equal.
+       apply finz_to_z_eq.
+       cbn.
+       solve_finz.
+    }
+    rewrite H in Heqc2. clear H.
     rewrite /fill_rx in Heqc2.
-    assert (Htemp : ∀ σ t r r1 i, get_vm_mail_box (copy_page_segment_unsafe σ t r r1) i =
+    assert (Htemp : ∀ σ dst ws i, get_vm_mail_box (write_mem_segment_unsafe σ dst ws) i =
                                   get_vm_mail_box σ i).
     f_equal.
     rewrite Htemp in Heqc2; clear Htemp.
-    assert (Hmb :  get_vm_mail_box σ1 i = (ptx, (rxp,None))).
+    assert (Hmb :  get_vm_mail_box σ1 i = (ptx, (prx,None))).
     { destruct (get_vm_mail_box σ1 i).
-    destruct r.
-    cbn in Htx ,Hrx2, Hrx1.
-    subst t0 o p.
-    reflexivity.
+      destruct r.
+      cbn in Htx ,Hrx2, Hrx1.
+      subst t0 o p.
+      reflexivity.
     }
     rewrite /get_tx_pid_global /get_rx_pid_global Hmb /=  in Heqc2.
-    rewrite fill_rx_unsafe_preserve_current_vm in Heqc2.
-    rewrite copy_page_segment_unsafe_preserve_current_vm in Heqc2.
-    rewrite Hcureq in Heqc2.
-    assert (Hcheck : (i =? i)%nat = true).
-    { by apply <- Nat.eqb_eq. }
+    assert (Hcheck: (i =? i)%nat = true).
+    { apply <- Nat.eqb_eq. reflexivity. }
     rewrite Hcheck in Heqc2.
-    pose proof Hretri1 as Hretri1''.
-    pose proof Hretri2 as Hretri2''.
+    pose proof Hretri1 as Hretri1'.
+    pose proof Hretri2 as Hretri2'.
     rewrite Htrans in Hretri1.
-    inversion Hretri1 as [Hretri1'].
-    rewrite -Hretri1' //= in Hretri2.
-    rewrite Hretri2 //= /transaction_write_rx /transaction_to_list_words /transaction_to_transaction_descriptor in Heqc2.
+    inversion Hretri1 as [Hretri1''].
+    rewrite -Hretri1'' //= in Hretri2.
+    subst b.
+    rewrite -Hretri1 in Hretri1'.
+    clear Hretri1.
     destruct c2 as [c21 c22].
-    destruct HstepP; subst m2 σ2; rewrite Heqc2.
+    destruct Htt as [[Htt ->]|[Htt ->]];subst tt;
+    rewrite/= in Heqc2;
+    destruct HstepP; subst m2 σ2; rewrite Heqc2;
     simpl;clear Heqc2.
-    rewrite /gen_vm_interp /update_incr_PC /update_reg.
-    rewrite update_offset_PC_preserve_hpool update_access_batch_preserve_hpool
-            update_reg_global_preserve_hpool update_transaction_preserve_hpool fill_rx_unsafe_preserve_hpool
-            copy_page_segment_unsafe_preserve_hpool.
-    iFrame "Hσhp".
-    rewrite update_offset_PC_preserve_tx update_access_batch_preserve_tx
-            update_reg_global_preserve_tx update_transaction_preserve_tx fill_rx_unsafe_preserve_tx.
-    2 : {
-      rewrite /get_tx_pid_global /get_vm_mail_box //= /get_mail_boxes.
-    }
-    rewrite copy_page_segment_unsafe_preserve_tx.
-    rewrite /get_tx_agree.
-    iFrame "Hσtx".
-    rewrite update_offset_PC_preserve_current_vm update_access_batch_preserve_current_vm
-            update_reg_global_preserve_current_vm update_transaction_preserve_current_vm
-            fill_rx_unsafe_preserve_current_vm copy_page_segment_unsafe_preserve_current_vm.
-    rewrite Hcureq.
-    iFrame "Hcur".
-    rewrite update_offset_PC_preserve_rx1 update_access_batch_preserve_rx1
-            update_reg_global_preserve_rx1 update_transaction_preserve_rx1.
-    rewrite fill_rx_unsafe_preserve_rx1.
-     2 : {
-       rewrite /get_rx_pid_global /get_vm_mail_box /get_mail_boxes //=.
-     }
-     rewrite copy_page_segment_unsafe_preserve_rx1.
-     iFrame "Hσrx1".
-    (* update regs *)
-    rewrite (update_offset_PC_update_PC1 _ i ai 1).
-    rewrite update_access_batch_preserve_regs update_reg_global_update_reg update_transaction_preserve_regs
-             fill_rx_unsafe_preserve_regs copy_page_segment_unsafe_preserve_regs; try solve_reg_lookup.
-    2:{
-      rewrite update_access_batch_preserve_current_vm update_reg_global_preserve_current_vm
-      update_transaction_preserve_current_vm fill_rx_unsafe_preserve_current_vm
-      copy_page_segment_unsafe_preserve_current_vm //.
-    }
-    2: {
-      rewrite update_access_batch_preserve_regs update_reg_global_update_reg.
-      rewrite update_transaction_preserve_regs
-             fill_rx_unsafe_preserve_regs copy_page_segment_unsafe_preserve_regs; try solve_reg_lookup.
-      rewrite lookup_insert_ne; [solve_reg_lookup|done].
-      exists r0.
-      rewrite update_transaction_preserve_regs
-             fill_rx_unsafe_preserve_regs copy_page_segment_unsafe_preserve_regs; try solve_reg_lookup.
-    }
-     iDestruct ((gen_reg_update2_global PC i _ (ai ^+ 1)%f R0 i _ (encode_hvc_ret_code Succ)) with "Hσreg PC Hr0")
-      as ">[Hσreg [PC Hr0]]";try f_equal.
-    { left;done. }
-     iFrame "Hσreg".
-    (* update page table *)
-    rewrite update_offset_PC_preserve_owned update_access_batch_preserve_ownerships
-            update_reg_global_preserve_owned update_transaction_preserve_owned
-            fill_rx_unsafe_preserve_owned copy_page_segment_unsafe_preserve_owned.
-    iFrame "Hσowned".
-    rewrite update_offset_PC_preserve_access.
-    rewrite (@update_access_batch_update_pagetable_union _ i sacc ExclusiveAccess spsd psd Hpsd); f_equal;eauto.
-    iDestruct ((gen_access_update_union spsd) with "HA Hσaccess") as ">[Hσaccess' HA']";f_equal.
-    {exact Hpsd. }
-    rewrite update_reg_global_preserve_access update_transaction_preserve_access
-    fill_rx_unsafe_preserve_access copy_page_segment_unsafe_preserve_access.
-    iFrame "Hσaccess'".
-    rewrite update_offset_PC_preserve_excl.
-    rewrite (@update_exclusive_batch_update_pagetable_union _ i sexcl spsd psd Hpsd);f_equal; eauto.
-    iDestruct ((gen_excl_update_union spsd) with "HE Hσexcl") as ">[Hσexcl' HE']"; f_equal.
-    { exact Hpsd. }
-    rewrite update_reg_global_preserve_excl update_transaction_preserve_excl
-    fill_rx_unsafe_preserve_excl copy_page_segment_unsafe_preserve_excl.
-    iFrame "Hσexcl'".
-    (* update transactions *)
-    rewrite -get_trans_gmap_preserve_dom.
-    rewrite update_offset_PC_preserve_trans update_access_batch_preserve_trans
-            update_reg_global_preserve_trans.
-    rewrite (@toggle_transaction_unsafe_preserve_trans _ _ b).
-    2 : {
-      cbn.
-      assumption.
-    }
-    rewrite fill_rx_unsafe_preserve_trans copy_page_segment_unsafe_preserve_trans.
-    iFrame "Htrans".
-      (* update rx *)
-    iCombine "HRX1 HRX2" as "HRX".
-    rewrite update_offset_PC_preserve_rx2 update_access_batch_preserve_rx2
-            update_reg_global_preserve_rx2 update_transaction_preserve_rx2.
-    iDestruct ((gen_rx_gmap_update_global_None i r1 i rxp) with "Hσrx2 HRX") as ">[Hσrx' [HRX1 HRX2]]".
-    rewrite fill_rx_unsafe_update_mailbox.
-    iFrame "Hσrx'".
-    (* update retri *)
-    rewrite update_offset_PC_preserve_mem update_access_batch_preserve_mem
-            update_reg_global_preserve_mem update_transaction_preserve_mem fill_rx_unsafe_preserve_mem.
-    iDestruct ((@gen_retri_update _ _ _ false true wh) with "Hwhf Hrcv") as ">[Hrcv' Hwhf']".
-    { subst b t.
-      eapply get_retri_gmap_lookup.
-      exact Hretri1''.
-    }
-    rewrite update_offset_PC_preserve_retri update_access_batch_preserve_retri
-    update_reg_global_preserve_retri /update_transaction /insert_transaction.
-    rewrite -get_retri_gmap_to_get_transaction fill_rx_unsafe_preserve_receivers
-    copy_page_segment_unsafe_preserve_receivers.
-    iFrame "Hrcv'".
-    rewrite update_offset_PC_preserve_trans' update_access_batch_preserve_trans'
-            update_reg_global_preserve_trans' /get_transactions /=.
-    (* update mem *)
-    rewrite /copy_page_segment_unsafe /copy_from_addr_to_addr_unsafe.
-    rewrite /mem_region.
-    assert (Hlength: ((read_mem_segment_unsafe σ1 ptx r1)) = des).
     {
-      rewrite /read_mem_segment_unsafe.
-      rewrite /get_mem in Hadesc.
-      apply (f_equal Z.to_nat) in Hdesl.
-      rewrite Hdesl.
-      rewrite Nat2Z.id.
-      clear Hdes Hdesl Hseq Hlendesclt Hmb.
-      generalize dependent (of_pid ptx).
-      induction des; first done.
-      simpl in IHdes.
-      simpl.
-      intros.
-      rewrite /get_memory_unsafe.
-      rewrite (Hadesc 0 f a).
-      simpl.
-      f_equal.
-      rewrite /get_memory_unsafe in IHdes.
-      rewrite (IHdes (f ^+ 1)%f).
-      reflexivity.
-      intros k y1 y2 H1 H2.
-      apply Hadesc with (S k); auto.
-      reflexivity.
-      reflexivity.
-    }
-    iDestruct "HRXCont" as "[%l0 [HRXCont' %Hlen']]".
-    rewrite Hlength.
-    rewrite /write_mem_segment_unsafe //.
-    cbn.
-    iDestruct ((gen_mem_update_SepL2 (finz.seq rxp (length l0)) l0 des) with "Hσmem HRXCont'")
-      as ">[Hσmem Hmem]".
-    { rewrite Hlen'.
-      apply finz_seq_NoDup'.
-      pose proof last_addr_in_bound as Hbound.
-      specialize (Hbound rxp).
-      solve_finz.
-    }
-    assumption.
-    assert ((zip (finz.seq rxp (length l0)) des) = (zip (finz.seq rxp (Z.to_nat 1000)) des)) as ->.
-    {
-      rewrite -finz_seq_zip_page;auto.
-      rewrite Hlen' //.
-      lia.
-    }
-    iFrame "Hσmem".
-    iSplitR.
-    iPureIntro.
-    split;[rewrite get_trans_gmap_preserve_dom // |].
-    apply map_Forall_insert_2; auto.
-    simpl.
-    rewrite <-Hlenl.
-    destruct (finz_spec word_size l) as [H _].
-    rewrite ->(reflect_iff _ _ (Z.ltb_spec0 l word_size)) in H.
-    assumption.
+    iDestruct ((retrieve_lend_share σ1 i Lending (sexcl ∪ spsd) ExclusiveAccess spsd psd)
+                 with "PC HA HE Hr0 Hwh Hwhf HRX1 HRX2 HRXCont [Hcur Hσmem Hσreg Hσtx Hσrx1 Hσrx2 Hσowned Hσaccess Hσexcl Htrans Hσhp Hrcv]") as ">[Hσ Hres]";try done.
+    left.
+    repeat split;done.
+    iFrame.
+    done.
+    iFrame "Hσ".
     iApply "HΦ".
-    rewrite Hlen'.
+    iFrame.
+    iDestruct "Hres" as "(?&?&?&?&?&?&?&?&?)".
+    rewrite Hdesrx.
     by iFrame.
+    }
+    {
+    iDestruct ((retrieve_lend_share σ1 i Sharing sexcl SharedAccess spsd psd)
+                 with "PC HA HE Hr0 Hwh Hwhf HRX1 HRX2 HRXCont [Hcur Hσmem Hσreg Hσtx Hσrx1 Hσrx2 Hσowned Hσaccess Hσexcl Htrans Hσhp Hrcv]") as ">[Hσ Hres]";try done.
+    right;done.
+    iFrame.
+    done.
+    iFrame "Hσ".
+    iApply "HΦ".
+    iFrame.
+    iDestruct "Hres" as "(?&?&?&?&?&?&?&?&?)".
+    rewrite Hdesrx.
+    by iFrame.
+    }
 Qed.
 
-(* TODO hvc_retreive_share *)
+
+Lemma hvc_retrieve_lend {wi sown sacc pi sexcl i j destx wf' desrx ptx prx l} {spsd: gset PID}
+      ai r0 r1 wh wf (psd: list PID) :
+  (* the current instruction is hvc *)
+  (* the decoding of wi is correct *)
+  decode_instruction wi = Some(Hvc) ->
+  (* the instruction is in page pi *)
+  addr_in_page ai pi ->
+  (* the decoding of R0 is FFA_LEND *)
+  decode_hvc_func r0 = Some(Retrieve) ->
+  (* pi page in spsd is accessible for VM i *)
+  pi ∈ sacc ->
+  (* spsd is the gset of all to-be-donated pages *)
+  spsd = (list_to_set psd) ->
+  spsd ## sacc ->
+  spsd ## sown ->
+  spsd ## sexcl ->
+  (finz.to_z l) = (Z.of_nat (length psd)) ->
+  destx = ([of_imm (encode_vmid j); wf'; wh ;of_imm (encode_vmid i)] ) ->
+  desrx = ([of_imm (encode_vmid j); wf; wh; encode_transaction_type Lending;l] ++ map of_pid psd) ->
+  (finz.to_z r1) = (Z.of_nat (length destx)) ->
+  seq_in_page (of_pid ptx) (length destx) ptx ->
+  seq_in_page (of_pid prx) (length desrx) prx ->
+  {SS{{ ▷(PC @@ i ->r ai) ∗ ▷ ai ->a wi ∗ ▷ A@i:={1}[sacc]
+  ∗ ▷ (R0 @@ i ->r r0) ∗ ▷ wh ->re false
+  ∗ ▷ (R1 @@ i ->r r1) ∗ ▷ wh ->t{1}(j, wf, i, psd, Lending)
+  ∗ ▷ O@i:={1}[sown] ∗ ▷ E@i:={1}[sexcl] ∗ ▷ TX@ i := ptx
+  ∗ ▷ mem_region destx ptx ∗ ▷ RX@ i :=( prx !) ∗ ▷ (∃l, mem_region l prx ∗ ⌜ length l = length desrx ⌝)}}}
+   ExecI @ i {{{ RET ExecI ; PC @@ i ->r (ai ^+ 1)%f ∗ ai ->a wi
+  ∗ O@i:={1}[(sown)] ∗ E@i:={1}[(sexcl ∪ spsd)] ∗ A@i:={1}[(sacc ∪ spsd)]
+  ∗ R0 @@ i ->r (encode_hvc_ret_code Succ) ∗ R1 @@ i ->r r1 ∗ wh ->t{1}(j, wf, i, psd, Lending)
+  ∗ wh ->re true ∗ TX@ i := ptx ∗ RX@ i :=( prx ! (l ^+ 5)%f, i)
+  ∗ mem_region destx ptx ∗ mem_region desrx prx }}}.
+Proof.
+  iIntros (???????????????).
+  iIntros "(?&?&?&?&?&?&?&?&?&?&?&?&?)".
+  iApply hvc_retrieve_lend_share;auto.
+  exact H0.
+  exact H1.
+  exact H2.
+  exact H8.
+  iFrame.
+Qed.
+
+Lemma hvc_retrieve_share { wi sown sacc pi sexcl i j destx wf' desrx ptx prx l} {spsd: gset PID}
+      ai r0 r1 wh wf (psd: list PID) :
+  (* the current instruction is hvc *)
+  (* the decoding of wi is correct *)
+  decode_instruction wi = Some(Hvc) ->
+  (* the instruction is in page pi *)
+  addr_in_page ai pi ->
+  (* the decoding of R0 is FFA_LEND *)
+  decode_hvc_func r0 = Some(Retrieve) ->
+  (* pi page in spsd is accessible for VM i *)
+  pi ∈ sacc ->
+  (* spsd is the gset of all to-be-donated pages *)
+  spsd = (list_to_set psd) ->
+  spsd ## sacc ->
+  spsd ## sown ->
+  spsd ## sexcl ->
+  (finz.to_z l) = (Z.of_nat (length psd)) ->
+  destx = ([of_imm (encode_vmid j); wf'; wh ;of_imm (encode_vmid i)] ) ->
+  desrx = ([of_imm (encode_vmid j); wf; wh; encode_transaction_type Sharing;l] ++ map of_pid psd) ->
+  (finz.to_z r1) = (Z.of_nat (length destx)) ->
+  seq_in_page (of_pid ptx) (length destx) ptx ->
+  seq_in_page (of_pid prx) (length desrx) prx ->
+  {SS{{ ▷(PC @@ i ->r ai) ∗ ▷ ai ->a wi ∗ ▷ A@i:={1}[sacc]
+  ∗ ▷ (R0 @@ i ->r r0) ∗ ▷ wh ->re false
+  ∗ ▷ (R1 @@ i ->r r1) ∗ ▷ wh ->t{1}(j, wf, i, psd, Sharing)
+  ∗ ▷ O@i:={1}[sown] ∗ ▷ E@i:={1}[sexcl] ∗ ▷ TX@ i := ptx
+  ∗ ▷ mem_region destx ptx ∗ ▷ RX@ i :=( prx !) ∗ ▷ (∃l, mem_region l prx ∗ ⌜ length l = length desrx ⌝)}}}
+   ExecI @ i {{{ RET ExecI ; PC @@ i ->r (ai ^+ 1)%f ∗ ai ->a wi
+  ∗ O@i:={1}[(sown)] ∗ E@i:={1}[sexcl] ∗ A@i:={1}[(sacc ∪ spsd)]
+  ∗ R0 @@ i ->r (encode_hvc_ret_code Succ) ∗ R1 @@ i ->r r1 ∗ wh ->t{1}(j, wf, i, psd, Sharing)
+  ∗ wh ->re true ∗ TX@ i := ptx ∗ RX@ i :=( prx ! (l ^+ 5)%f, i)
+  ∗ mem_region destx ptx ∗ mem_region desrx prx }}}.
+Proof.
+  iIntros (???????????????).
+  iIntros "(?&?&?&?&?&?&?&?&?&?&?&?&?)".
+  iApply hvc_retrieve_lend_share;auto.
+  exact H0.
+  exact H1.
+  exact H2.
+  exact H8.
+  iFrame.
+Qed.
 
 End retrieve.
